Introduce rust_lang

nola/examples/ilist.v
@@ -1,11 +1,11 @@
 (** * Infinite shared mutable linked list examples *)
 
 From nola.examples Require Export con.
-From nola.heap_lang Require Export notation proofmode.
+From nola.rust_lang Require Export notation proofmode.
 Import FunPRNotation WpwNotation DsemNotation.
 
 Section ilist.
-  Context `{!heapGS_gen hlc Σ, !SemCifcon JUDG CON Σ, !Jsem JUDG (iProp Σ),
+  Context `{!lrustGS_gen hlc Σ, !SemCifcon JUDG CON Σ, !Jsem JUDG (iProp Σ),
     !inv'GS (cifOF CON) Σ, !InvCon CON, !InvSem JUDG CON Σ}.
   Implicit Type (Px Qx : cif CON Σ) (Φx Ψx : loc → cif CON Σ) (l : loc).
 
@@ -60,85 +60,87 @@ Section ilist.
   Proof. apply ne_proper, _. Qed.
 
   (** Access the tail of a list *)
-  Definition tail_ilist : val := λ: "l", !("l" +ₗ #1).
+  Definition tail_ilist : val := λ: ["l"], !ˢᶜ("l" +ₗ #1).
   Lemma twp_tail_list {N E Φx l} : ↑N ⊆ E →
     [[{ ilist N Φx l }]][inv_wsat ⟦⟧]
-      tail_ilist #l @ E
+      tail_ilist [ #l] @ E
     [[{ l', RET #l'; ilist N Φx l' }]].
   Proof.
-    iIntros (? Ψ) "/= [_ #itl] →Ψ". wp_rec. wp_pure.
+    iIntros (? Ψ) "/= [_ #itl] →Ψ". wp_rec. wp_op.
     iMod (inv_tok_acc with "itl") as "/=[(%l' & >↦l' & ltl) cl]"; [done|].
-    rewrite sem_ilist. iDestruct "ltl" as "#ltl".
-    wp_load. iModIntro. iMod ("cl" with "[$↦l']") as "_".
-    { by rewrite sem_ilist. }
+    rewrite sem_ilist. iDestruct "ltl" as "#ltl". wp_read.
+    iMod ("cl" with "[$↦l']") as "_". { by rewrite sem_ilist. }
     iModIntro. iApply ("→Ψ" with "ltl").
   Qed.
 
   (** Iterate over a list *)
-  Definition iter_ilist : val := rec: "self" "f" "c" "l" :=
-    if: !"c" ≤ #0 then #() else
-      "f" "l";; "c" <- !"c" - #1;; "self" "f" "c" (tail_ilist "l").
+  Definition iter_ilist : val := rec: "self" ["f"; "c"; "l"] :=
+    if: !"c" ≤ #0 then #☠ else
+      "f" ["l"];; "c" <- !"c" - #1;; "self" ["f"; "c"; tail_ilist ["l"]].
   Lemma twp_iter_list {N E Φx c l} {f : val} {n : nat} : ↑N ⊆ E →
-    (∀ l', [[{ inv_tok N (Φx l') }]][inv_wsat ⟦⟧] f #l' @ E
-      [[{ RET #(); True }]]) -∗
+    (∀ l', [[{ inv_tok N (Φx l') }]][inv_wsat ⟦⟧] f [ #l'] @ E
+      [[{ RET #☠; True }]]) -∗
     [[{ c ↦ #n ∗ ilist N Φx l }]][inv_wsat ⟦⟧]
-      iter_ilist f #c #l @ E
-    [[{ RET #(); c ↦ #0 }]].
+      iter_ilist [f; #c; #l] @ E
+    [[{ RET #☠; c ↦ #0 }]].
   Proof.
     iIntros "% #f /=" (Ψ) "!> [c↦ #l] →Ψ".
     iInduction n as [|m] "IH" forall (l) "l".
-    { wp_rec. wp_load. wp_pures. by iApply "→Ψ". }
-    wp_rec. wp_load. wp_pures. wp_apply "f".
+    { wp_rec. wp_read. wp_op. wp_if. by iApply "→Ψ". }
+    wp_rec. wp_read. wp_op. wp_if. wp_apply "f".
     { iDestruct "l" as "[$ _]". }
-    iIntros "_". wp_load. wp_store. have -> : (S m - 1)%Z = m by lia.
+    iIntros "_". wp_seq. wp_read. wp_op. wp_write.
+    have -> : (S m - 1)%Z = m by lia.
     wp_apply twp_tail_list; [done..|]. iIntros (l') "#ltl".
     iApply ("IH" with "c↦ →Ψ ltl").
   Qed.
 
   (** Iterate over a list with two threads *)
   Lemma twp_fork_iter_list {N E Φx c' c l} {f : val} {m n : nat} : ↑N ⊆ E →
-    (∀ l', [[{ inv_tok N (Φx l') }]][inv_wsat ⟦⟧] f #l' @ E
-      [[{ RET #(); True }]]) -∗
+    (∀ l', [[{ inv_tok N (Φx l') }]][inv_wsat ⟦⟧] f [ #l'] @ E
+      [[{ RET #☠; True }]]) -∗
     [[{ c' ↦ #m ∗ c ↦ #n ∗ ilist N Φx l }]][inv_wsat ⟦⟧]
-      Fork (iter_ilist f #c' #l);; iter_ilist f #c #l @ E
-    [[{ RET #(); c ↦ #0 }]].
+      Fork (iter_ilist [f; #c'; #l]);; iter_ilist [f; #c; #l] @ E
+    [[{ RET #☠; c ↦ #0 }]].
   Proof.
     iIntros "% #f" (Ψ) "!> (↦' & ↦ & #l) →Ψ". wp_apply (twp_fork with "[↦']").
     { iApply (twp_mask_mono _ E); [done|].
       wp_apply (twp_iter_list with "f [$↦' $l //]"); [done|]. by iIntros. }
-    wp_pures. by wp_apply (twp_iter_list with "f [$↦ $l //]").
+    iIntros. wp_seq. by wp_apply (twp_iter_list with "f [$↦ $l //]").
   Qed.
 
   (** Iterate over an unbounded number of elements of a list with an unbounded
     number of threads *)
-  Definition forks_iter_list : val := rec: "self" "f" "k" "l" :=
-    if: !"k" ≤ #0 then #() else
-      Fork (let: "c" := ref Ndnat in iter_ilist "f" "c" "l");;
-      "k" <- !"k" - #1;; "self" "f" "k" "l".
+  Definition forks_iter_list : val := rec: "self" ["f"; "k"; "l"] :=
+    if: !"k" ≤ #0 then #☠ else
+      Fork (let: "c" := Alloc #1 in "c" <- Ndnat;; iter_ilist ["f"; "c"; "l"]);;
+      "k" <- !"k" - #1;; "self" ["f"; "k"; "l"].
   Lemma twp_forks_iter_list {N E Φx k l} {f : val} {n : nat} :
-    (∀ l', [[{ inv_tok N (Φx l') }]][inv_wsat ⟦⟧] f #l'
-      [[{ RET #(); True }]]) -∗
+    (∀ l', [[{ inv_tok N (Φx l') }]][inv_wsat ⟦⟧] f [ #l']
+      [[{ RET #☠; True }]]) -∗
     [[{ k ↦ #n ∗ ilist N Φx l }]][inv_wsat ⟦⟧]
-      forks_iter_list f #k #l @ E
-    [[{ RET #(); k ↦ #0 }]].
+      forks_iter_list [f; #k; #l] @ E
+    [[{ RET #☠; k ↦ #0 }]].
   Proof.
     iIntros "#f" (Ψ) "!> [↦ #l] →Ψ". iInduction n as [|m] "IH" forall (l) "l".
-    { wp_rec. wp_load. wp_pures. by iApply "→Ψ". }
-    wp_rec. wp_load. wp_pures. wp_apply twp_fork.
-    { wp_apply twp_ndnat; [done|]. iIntros (?) "_". wp_alloc c as "↦".
-      wp_pures. wp_apply (twp_iter_list with "f [$↦ $l //]"); by [|iIntros]. }
-    wp_load. wp_op. have -> : (S m - 1)%Z = m by lia. wp_store.
+    { wp_rec. wp_read. wp_op. wp_if. by iApply "→Ψ". }
+    wp_rec. wp_read. wp_op. wp_if. wp_apply twp_fork.
+    { wp_alloc c as "↦" "†". rewrite heap_pointsto_vec_singleton. wp_let.
+      wp_apply twp_ndnat; [done|]. iIntros (?) "_". wp_write.
+      wp_apply (twp_iter_list with "f [$↦ $l //]"); by [|iIntros]. }
+    iIntros. wp_seq. wp_read. wp_op. have -> : (S m - 1)%Z = m by lia. wp_write.
     iApply ("IH" with "↦ →Ψ l").
   Qed.
   Lemma twp_nd_forks_iter_list {N E Φx l} {f : val} :
-    (∀ l', [[{ inv_tok N (Φx l') }]][inv_wsat ⟦⟧] f #l'
-      [[{ RET #(); True }]]) -∗
+    (∀ l', [[{ inv_tok N (Φx l') }]][inv_wsat ⟦⟧] f [ #l']
+      [[{ RET #☠; True }]]) -∗
     [[{ ilist N Φx l }]][inv_wsat ⟦⟧]
-      let: "k" := ref Ndnat in forks_iter_list f "k" #l @ E
-    [[{ RET #(); True }]].
+      let: "k" := Alloc #1 in "k" <- Ndnat;; forks_iter_list [f; "k"; #l] @ E
+    [[{ RET #☠; True }]].
   Proof.
-    iIntros "#f" (Ψ) "!> #l →Ψ". wp_apply twp_ndnat; [done|]. iIntros (?) "_".
-    wp_alloc k as "↦". wp_pures.
+    iIntros "#f" (Ψ) "!> #l →Ψ". wp_alloc k as "↦" "†".
+    rewrite heap_pointsto_vec_singleton. wp_let. wp_apply twp_ndnat; [done|].
+    iIntros (?) "_". wp_write.
     wp_apply (twp_forks_iter_list with "f [$↦ $l //]"). iIntros "_".
     by iApply "→Ψ".
   Qed.
