nola/examples/borrow.v
@@ -1,12 +1,12 @@
 (** * Borrow examples *)
 
 From nola.examples Require Export nsynty con.
-From nola.heap_lang Require Export notation proofmode.
+From nola.rust_lang Require Export notation proofmode.
 Import ProdNotation FunPRNotation UpdwNotation WpwNotation DsemNotation
   LftNotation ProphNotation NsyntyNotation.
 
 Section borrow.
-  Context `{!heapGS_gen hlc Σ, !SemCifcon JUDG CON Σ, !Jsem JUDG (iProp Σ),
+  Context `{!lrustGS_gen hlc Σ, !SemCifcon JUDG CON Σ, !Jsem JUDG (iProp Σ),
     !inv'GS (cifOF CON) Σ, !InvCon CON, !InvSem JUDG CON Σ,
     !pborrowGS nsynty (cifOF CON) Σ, !BorCon CON, !BorSem JUDG CON Σ}.
   Implicit Type (Px Qx : cif CON Σ) (Φx Ψx : loc → cif CON Σ) (l : loc).
@@ -21,7 +21,7 @@ Section borrow.
   Proof.
     iIntros (Ψ) "(#⊑ & [β β'] & b) →Ψ".
     iMod (nbor_tok_open (M:=bupd_0) with "β b") as "/=[o [%l'[>↦ b']]]".
-    iApply twpw_fupdw_nonval; [done|]. wp_load. iModIntro.
+    iApply twpw_fupdw_nonval; [done|]. wp_read.
     iMod (lft_sincl_live_acc with "⊑ β'") as (?) "[α →β']".
     rewrite sem_ecustom /=.
     iMod (nbor_tok_reborrow (M:=bupd_0) with "⊑ α b'") as "(α & →b' & b')".
@@ -49,7 +49,7 @@ Section borrow.
   Proof.
     iIntros (Ψ) "(#⊑ & [β β'] & b) →Ψ".
     iMod (pbor_tok_open (M:=bupd_0) with "β b") as "/=[o[%l'[>↦ b']]]".
-    iApply twpw_fupdw_nonval; [done|]. wp_load. iModIntro.
+    iApply twpw_fupdw_nonval; [done|]. wp_read.
     iMod (lft_sincl_live_acc with "⊑ β'") as (?) "[α →β']".
     rewrite sem_ecustom /=.
     iMod (pobor_pbor_tok_reborrow (TY:=nsynty) (M:=bupd_0)
@@ -62,13 +62,12 @@ Section borrow.
   Lemma imbor_load {l α q} {n : Z} :
     [[{ q.[α] ∗ inv_tok nroot (cif_bor α (▷ l ↦ #n)) }]]
       [inv_wsat ⟦⟧ ∗ pborrow_wsat bupd_0 ⟦⟧]
-      !#l
+      !ˢᶜ#l
     [[{ RET #n; q.[α] }]].
   Proof.
     iIntros (Φ) "[α #i] →Φ". iMod (inv_tok_acc with "i") as "/=[b cl]"; [done|].
     rewrite sem_ecustom /=.
-    iMod (nbor_tok_open (M:=bupd_0) with "α b") as "/=[o >↦]". wp_load.
-    iModIntro.
+    iMod (nbor_tok_open (M:=bupd_0) with "α b") as "/=[o >↦]". wp_read.
     iMod (nobor_tok_close (M:=bupd_0) with "o [↦]") as "[α b]"=>/=; [done|].
     iMod ("cl" with "b") as "_". iModIntro. by iApply "→Φ".
   Qed.
