nola/rust_lang/adequacy.v
@@ -1,0 +1,57 @@
+From iris.program_logic Require Export adequacy weakestpre.
+From iris.algebra Require Import auth.
+From nola.rust_lang Require Export heap.
+From nola.rust_lang Require Import proofmode notation.
+From iris.prelude Require Import options.
+Import WpwNotation.
+
+Class lrustGpreS Σ := HeapGpreS {
+  lrustGpreS_inv :: invGpreS Σ;
+  lrustGpreS_heap :: inG Σ (authR heapUR);
+  lrustGpreS_heap_freeable :: inG Σ (authR heap_freeableUR)
+}.
+
+Definition lrustΣ : gFunctors :=
+  #[invΣ;
+    GFunctor (constRF (authR heapUR));
+    GFunctor (constRF (authR heap_freeableUR))].
+Global Instance subG_lrustGpreS {Σ} : subG lrustΣ Σ → lrustGpreS Σ.
+Proof. solve_inG. Qed.
+
+(** Partial correctness adequacy *)
+Definition lrust_adequacy Σ `{!lrustGpreS Σ} hlc e σ φ :
+  (∀ `{!lrustGS_gen hlc Σ}, ⊢ |={⊤}=>
+    ∃ W : iProp Σ, W ∗ WP[W] e {{ v, ⌜φ v⌝ }}) →
+  adequate NotStuck e σ (λ v _, φ v).
+Proof.
+  move=> big. apply adequate_alt=> ?? /erased_steps_nsteps[?[??]].
+  eapply (wpw_strong_adequacy_gen hlc Σ _); [|done]=> Hinv.
+  iMod (own_alloc (● to_heap σ)) as (vγ) "?".
+  { apply (auth_auth_valid (to_heap _)), to_heap_valid. }
+  iMod (own_alloc (● (∅ : heap_freeableUR))) as (fγ) "?";
+    first by apply auth_auth_valid.
+  set Hheap := HeapGS _ _ _ vγ fγ.
+  iMod (big (LRustGS _ _ Hinv Hheap)) as (W) "[??]". iModIntro.
+  iExists _, [_], _, _, _=>/=. iFrame. iSplit; [done|].
+  iIntros (??->??) "_ _ H _". iApply fupd_mask_intro_discard; [done|].
+  iSplit; [|done].
+  iDestruct (big_sepL2_cons_inv_r with "H") as (?? ->) "[? H]".
+  iDestruct (big_sepL2_nil_inv_r with "H") as %->. iIntros (??[=-><-]).
+  by rewrite to_of_val.
+Qed.
+
+(** Termination adequacy *)
+Theorem lrust_total Σ `{!lrustGpreS Σ} s e σ φ :
+  (∀ `{!lrustGS_gen HasNoLc Σ}, ⊢ |={⊤}=>
+    ∃ W : iProp Σ, W ∗ WP[W] e @ s; ⊤ [{ v, ⌜φ v⌝ }]) →
+  sn erased_step ([e], σ).
+Proof.
+  move=> big. eapply (twpw_total _ _ _ _ _ _ 0)=> Hinv.
+  iMod (own_alloc (● to_heap σ)) as (vγ) "?".
+  { apply (auth_auth_valid (to_heap _)), to_heap_valid. }
+  iMod (own_alloc (● (∅ : heap_freeableUR))) as (fγ) "?";
+    first by apply auth_auth_valid.
+  set Hheap := HeapGS _ _ _ vγ fγ.
+  iMod (big (LRustGS _ _ Hinv Hheap)) as (W) "[??]". iModIntro.
+  iExists _, _, _, _, _. by iFrame.
+Qed.
