nola/rust_lang/lang.v
@@ -1,0 +1,653 @@
+From iris.program_logic Require Export language ectx_language ectxi_language.
+From stdpp Require Export strings binders.
+From stdpp Require Import gmap.
+From iris.prelude Require Import options.
+
+Global Open Scope Z_scope.
+
+(** Expressions and vals. *)
+Definition block : Set := positive.
+Definition loc : Set := block * Z.
+
+Declare Scope loc_scope.
+Bind Scope loc_scope with loc.
+Delimit Scope loc_scope with L.
+Global Open Scope loc_scope.
+
+Inductive base_lit : Set :=
+| LitPoison | LitLoc (l : loc) | LitInt (n : Z).
+Inductive bin_op : Set :=
+| PlusOp | MinusOp | LeOp | EqOp | OffsetOp.
+Inductive order : Set :=
+| ScOrd | Na1Ord | Na2Ord.
+
+Notation "[ ]" := (@nil binder) : binder_scope.
+Notation "a :: b" := (@cons binder a%binder b%binder)
+  (at level 60, right associativity) : binder_scope.
+Notation "[ x1 ; x2 ; .. ; xn ]" :=
+  (@cons binder x1%binder (@cons binder x2%binder
+        (..(@cons binder xn%binder (@nil binder))..))) : binder_scope.
+Notation "[ x ]" := (@cons binder x%binder (@nil binder)) : binder_scope.
+
+Inductive expr :=
+| Var (x : string)
+| Lit (l : base_lit)
+| Rec (f : binder) (xl : list binder) (e : expr)
+| BinOp (op : bin_op) (e1 e2 : expr)
+| App (e : expr) (el : list expr)
+| Read (o : order) (e : expr)
+| Write (o : order) (e1 e2: expr)
+| CAS (e0 e1 e2 : expr)
+| Alloc (e : expr)
+| Free (e1 e2 : expr)
+| Case (e : expr) (el : list expr)
+| Fork (e : expr)
+| Ndnat.
+
+Global Arguments App _%_E _%_E.
+Global Arguments Case _%_E _%_E.
+
+Fixpoint is_closed (X : list string) (e : expr) : bool :=
+  match e with
+  | Var x => bool_decide (x ∈ X)
+  | Lit _ => true
+  | Rec f xl e => is_closed (f :b: xl +b+ X) e
+  | BinOp _ e1 e2 | Write _ e1 e2 | Free e1 e2 =>
+    is_closed X e1 && is_closed X e2
+  | App e el | Case e el => is_closed X e && forallb (is_closed X) el
+  | Read _ e | Alloc e | Fork e => is_closed X e
+  | CAS e0 e1 e2 => is_closed X e0 && is_closed X e1 && is_closed X e2
+  | Ndnat => true
+  end.
+
+Class Closed (X : list string) (e : expr) := closed : is_closed X e.
+Global Instance closed_proof_irrel env e : ProofIrrel (Closed env e).
+Proof. rewrite /Closed. apply _. Qed.
+Global Instance closed_decision env e : Decision (Closed env e).
+Proof. rewrite /Closed. apply _. Qed.
+
+Inductive val :=
+| LitV (l : base_lit)
+| RecV (f : binder) (xl : list binder) (e : expr) `{!Closed (f :b: xl +b+ []) e}.
+
+Bind Scope val_scope with val.
+
+Definition of_val (v : val) : expr :=
+  match v with
+  | RecV f x e => Rec f x e
+  | LitV l => Lit l
+  end.
+
+Definition to_val (e : expr) : option val :=
+  match e with
+  | Rec f xl e =>
+    if decide (Closed (f :b: xl +b+ []) e) then Some (RecV f xl e) else None
+  | Lit l => Some (LitV l)
+  | _ => None
+  end.
+
+(** The state: heaps of vals*lockstate. *)
+Inductive lock_state :=
+| WSt | RSt (n : nat).
+Definition state := gmap loc (lock_state * val).
+
+(** Evaluation contexts *)
+Inductive ectx_item :=
+| BinOpLCtx (op : bin_op) (e2 : expr)
+| BinOpRCtx (op : bin_op) (v1 : val)
+| AppLCtx (e2 : list expr)
+| AppRCtx (v : val) (vl : list val) (el : list expr)
+| ReadCtx (o : order)
+| WriteLCtx (o : order) (e2 : expr)
+| WriteRCtx (o : order) (v1 : val)
+| CasLCtx (e1 e2: expr)
+| CasMCtx (v0 : val) (e2 : expr)
+| CasRCtx (v0 : val) (v1 : val)
+| AllocCtx
+| FreeLCtx (e2 : expr)
+| FreeRCtx (v1 : val)
+| CaseCtx (el : list expr).
+
+Definition fill_item (Ki : ectx_item) (e : expr) : expr :=
+  match Ki with
+  | BinOpLCtx op e2 => BinOp op e e2
+  | BinOpRCtx op v1 => BinOp op (of_val v1) e
+  | AppLCtx e2 => App e e2
+  | AppRCtx v vl el => App (of_val v) ((of_val <$> vl) ++ e :: el)
+  | ReadCtx o => Read o e
+  | WriteLCtx o e2 => Write o e e2
+  | WriteRCtx o v1 => Write o (of_val v1) e
+  | CasLCtx e1 e2 => CAS e e1 e2
+  | CasMCtx v0 e2 => CAS (of_val v0) e e2
+  | CasRCtx v0 v1 => CAS (of_val v0) (of_val v1) e
+  | AllocCtx => Alloc e
+  | FreeLCtx e2 => Free e e2
+  | FreeRCtx v1 => Free (of_val v1) e
+  | CaseCtx el => Case e el
+  end.
+
+(** Substitution *)
+Fixpoint subst (x : string) (es : expr) (e : expr)  : expr :=
+  match e with
+  | Var y => if bool_decide (y = x) then es else Var y
+  | Lit l => Lit l
+  | Rec f xl e =>
+    Rec f xl $ if bool_decide (BNamed x ≠ f ∧ BNamed x ∉ xl) then subst x es e else e
+  | BinOp op e1 e2 => BinOp op (subst x es e1) (subst x es e2)
+  | App e el => App (subst x es e) (map (subst x es) el)
+  | Read o e => Read o (subst x es e)
+  | Write o e1 e2 => Write o (subst x es e1) (subst x es e2)
+  | CAS e0 e1 e2 => CAS (subst x es e0) (subst x es e1) (subst x es e2)
+  | Alloc e => Alloc (subst x es e)
+  | Free e1 e2 => Free (subst x es e1) (subst x es e2)
+  | Case e el => Case (subst x es e) (map (subst x es) el)
+  | Fork e => Fork (subst x es e)
+  | Ndnat => Ndnat
+  end.
+
+Definition subst' (mx : binder) (es : expr) : expr → expr :=
+  match mx with BNamed x => subst x es | BAnon => id end.
+
+Fixpoint subst_l (xl : list binder) (esl : list expr) (e : expr) : option expr :=
+  match xl, esl with
+  | [], [] => Some e
+  | x::xl, es::esl => subst' x es <$> subst_l xl esl e
+  | _, _ => None
+  end.
+Global Arguments subst_l _%_binder _ _%_E.
+
+Definition subst_v (xl : list binder) (vsl : vec val (length xl))
+                   (e : expr) : expr :=
+  Vector.fold_right2 (λ b, subst' b ∘ of_val) e _ (list_to_vec xl) vsl.
+Global Arguments subst_v _%_binder _ _%_E.
+
+Lemma subst_v_eq (xl : list binder) (vsl : vec val (length xl)) e :
+  Some $ subst_v xl vsl e = subst_l xl (of_val <$> vec_to_list vsl) e.
+Proof.
+  revert vsl. induction xl as [|x xl IHxl]=>/= vsl; inv_vec vsl=>//=v vsl.
+  by rewrite -IHxl.
+Qed.
+
+(** The stepping relation *)
+(* Be careful to make sure that poison is always stuck when used for anything
+   except for reading from or writing to memory! *)
+Definition lit_of_bool (b : bool) : base_lit :=
+  LitInt $ Z.b2z b.
+
+Definition shift_loc (l : loc) (z : Z) : loc := (l.1, l.2 + z).
+
+Notation "l +ₗ z" := (shift_loc l%L z%Z)
+  (at level 50, left associativity) : loc_scope.
+
+Fixpoint init_mem (l:loc) (n:nat) (σ:state) : state :=
+  match n with
+  | O => σ
+  | S n => <[l:=(RSt 0, LitV LitPoison)]>(init_mem (l +ₗ 1) n σ)
+  end.
+
+Fixpoint free_mem (l:loc) (n:nat) (σ:state) : state :=
+  match n with
+  | O => σ
+  | S n => delete l (free_mem (l +ₗ 1) n σ)
+  end.
+
+Inductive lit_eq (σ : state) : base_lit → base_lit → Prop :=
+(* No refl case for poison *)
+| IntRefl z : lit_eq σ (LitInt z) (LitInt z)
+| LocRefl l : lit_eq σ (LitLoc l) (LitLoc l)
+(* Comparing unallocated pointers can non-deterministically say they are equal
+   even if they are not.  Given that our `free` actually makes addresses
+   re-usable, this may not be strictly necessary, but it is the most
+   conservative choice that avoids UB (and we cannot use UB as this operation is
+   possible in safe Rust).  See
+   <https://internals.rust-lang.org/t/comparing-dangling-pointers/3019> for some
+   more background. *)
+| LocUnallocL l1 l2 :
+    σ !! l1 = None →
+    lit_eq σ (LitLoc l1) (LitLoc l2)
+| LocUnallocR l1 l2 :
+    σ !! l2 = None →
+    lit_eq σ (LitLoc l1) (LitLoc l2).
+
+Inductive lit_neq : base_lit → base_lit → Prop :=
+| IntNeq z1 z2 :
+    z1 ≠ z2 → lit_neq (LitInt z1) (LitInt z2)
+| LocNeq l1 l2 :
+    l1 ≠ l2 → lit_neq (LitLoc l1) (LitLoc l2)
+| LocNeqNullR l :
+    lit_neq (LitLoc l) (LitInt 0)
+| LocNeqNullL l :
+    lit_neq (LitInt 0) (LitLoc l).
+
+Inductive bin_op_eval (σ : state) : bin_op → base_lit → base_lit → base_lit → Prop :=
+| BinOpPlus z1 z2 :
+    bin_op_eval σ PlusOp (LitInt z1) (LitInt z2) (LitInt (z1 + z2))
+| BinOpMinus z1 z2 :
+    bin_op_eval σ MinusOp (LitInt z1) (LitInt z2) (LitInt (z1 - z2))
+| BinOpLe z1 z2 :
+    bin_op_eval σ LeOp (LitInt z1) (LitInt z2) (lit_of_bool $ bool_decide (z1 ≤ z2))
+| BinOpEqTrue l1 l2 :
+    lit_eq σ l1 l2 → bin_op_eval σ EqOp l1 l2 (lit_of_bool true)
+| BinOpEqFalse l1 l2 :
+    lit_neq l1 l2 → bin_op_eval σ EqOp l1 l2 (lit_of_bool false)
+| BinOpOffset l z :
+    bin_op_eval σ OffsetOp (LitLoc l) (LitInt z) (LitLoc $ l +ₗ z).
+
+Definition stuck_term := App (Lit $ LitInt 0) [].
+
+Inductive base_step : expr → state → list Empty_set → expr → state → list expr → Prop :=
+| BinOpS op l1 l2 l' σ :
+    bin_op_eval σ op l1 l2 l' →
+    base_step (BinOp op (Lit l1) (Lit l2)) σ [] (Lit l') σ []
+| BetaS f xl e e' el σ:
+    Forall (λ ei, is_Some (to_val ei)) el →
+    Closed (f :b: xl +b+ []) e →
+    subst_l (f::xl) (Rec f xl e :: el) e = Some e' →
+    base_step (App (Rec f xl e) el) σ [] e' σ []
+| ReadScS l n v σ:
+    σ !! l = Some (RSt n, v) →
+    base_step (Read ScOrd (Lit $ LitLoc l)) σ [] (of_val v) σ []
+| ReadNa1S l n v σ:
+    σ !! l = Some (RSt n, v) →
+    base_step (Read Na1Ord (Lit $ LitLoc l)) σ
+              []
+              (Read Na2Ord (Lit $ LitLoc l)) (<[l:=(RSt $ S n, v)]>σ)
+              []
+| ReadNa2S l n v σ:
+    σ !! l = Some (RSt $ S n, v) →
+    base_step (Read Na2Ord (Lit $ LitLoc l)) σ
+              []
+              (of_val v) (<[l:=(RSt n, v)]>σ)
+              []
+| WriteScS l e v v' σ:
+    to_val e = Some v →
+    σ !! l = Some (RSt 0, v') →
+    base_step (Write ScOrd (Lit $ LitLoc l) e) σ
+              []
+              (Lit LitPoison) (<[l:=(RSt 0, v)]>σ)
+              []
+| WriteNa1S l e v v' σ:
+    to_val e = Some v →
+    σ !! l = Some (RSt 0, v') →
+    base_step (Write Na1Ord (Lit $ LitLoc l) e) σ
+              []
+              (Write Na2Ord (Lit $ LitLoc l) e) (<[l:=(WSt, v')]>σ)
+              []
+| WriteNa2S l e v v' σ:
+    to_val e = Some v →
+    σ !! l = Some (WSt, v') →
+    base_step (Write Na2Ord (Lit $ LitLoc l) e) σ
+              []
+              (Lit LitPoison) (<[l:=(RSt 0, v)]>σ)
+              []
+| CasFailS l n e1 lit1 e2 lit2 litl σ :
+    to_val e1 = Some $ LitV lit1 → to_val e2 = Some $ LitV lit2 →
+    σ !! l = Some (RSt n, LitV litl) →
+    lit_neq lit1 litl →
+    base_step (CAS (Lit $ LitLoc l) e1 e2) σ [] (Lit $ lit_of_bool false) σ  []
+| CasSucS l e1 lit1 e2 lit2 litl σ :
+    to_val e1 = Some $ LitV lit1 → to_val e2 = Some $ LitV lit2 →
+    σ !! l = Some (RSt 0, LitV litl) →
+    lit_eq σ lit1 litl →
+    base_step (CAS (Lit $ LitLoc l) e1 e2) σ
+              []
+              (Lit $ lit_of_bool true) (<[l:=(RSt 0, LitV lit2)]>σ)
+              []
+(* A succeeding CAS has to detect concurrent non-atomic read accesses, and
+   trigger UB if there is one.  In lambdaRust, succeeding and failing CAS are
+   not mutually exclusive, so it could happen that a CAS can both fail (and
+   hence not be stuck) but also succeed (and hence be racing with a concurrent
+   non-atomic read).  In that case, we have to explicitly reduce to a stuck
+   state; due to the possibility of failing CAS, we cannot rely on the current
+   state being stuck like we could in a language where failing and succeeding
+   CAS are mutually exclusive.
+
+   This means that CAS is atomic (it always reducs to an irreducible
+   expression), but not strongly atomic (it does not always reduce to a value).
+
+   If there is a concurrent non-atomic write, the CAS itself is stuck: All its
+   reductions are blocked.  *)
+| CasStuckS l n e1 lit1 e2 lit2 litl σ :
+    to_val e1 = Some $ LitV lit1 → to_val e2 = Some $ LitV lit2 →
+    σ !! l = Some (RSt n, LitV litl) → 0 < n →
+    lit_eq σ lit1 litl →
+    base_step (CAS (Lit $ LitLoc l) e1 e2) σ
+              []
+              stuck_term σ
+              []
+| AllocS n l σ :
+    0 < n →
+    (∀ m, σ !! (l +ₗ m) = None) →
+    base_step (Alloc $ Lit $ LitInt n) σ
+              []
+              (Lit $ LitLoc l) (init_mem l (Z.to_nat n) σ)
+              []
+| FreeS n l σ :
+    0 < n →
+    (∀ m, is_Some (σ !! (l +ₗ m)) ↔ 0 ≤ m < n) →
+    base_step (Free (Lit $ LitInt n) (Lit $ LitLoc l)) σ
+              []
+              (Lit LitPoison) (free_mem l (Z.to_nat n) σ)
+              []
+| CaseS i el e σ :
+    0 ≤ i →
+    el !! (Z.to_nat i) = Some e →
+    base_step (Case (Lit $ LitInt i) el) σ [] e σ []
+| ForkS e σ:
+    base_step (Fork e) σ [] (Lit LitPoison) σ [e]
+| NdnatS (n : nat) σ :
+    base_step Ndnat σ [] (Lit $ LitInt n) σ [].
+
+(** Basic properties about the language *)
+Lemma to_of_val v : to_val (of_val v) = Some v.
+Proof.
+  by induction v; simplify_option_eq; repeat f_equal; try apply (proof_irrel _).
+Qed.
+
+Lemma of_to_val e v : to_val e = Some v → of_val v = e.
+Proof.
+  revert v; induction e; intros v ?; simplify_option_eq; auto with f_equal.
+Qed.
+
+Global Instance of_val_inj : Inj (=) (=) of_val.
+Proof. by intros ?? Hv; apply (inj Some); rewrite -!to_of_val Hv. Qed.
+
+Global Instance fill_item_inj Ki : Inj (=) (=) (fill_item Ki).
+Proof. destruct Ki; intros ???; simplify_eq/=; auto with f_equal. Qed.
+
+Lemma fill_item_val Ki e :
+  is_Some (to_val (fill_item Ki e)) → is_Some (to_val e).
+Proof. intros [v ?]. destruct Ki; simplify_option_eq; eauto. Qed.
+
+Lemma val_stuck e1 σ1 κ e2 σ2 ef :
+  base_step e1 σ1 κ e2 σ2 ef → to_val e1 = None.
+Proof. destruct 1; naive_solver. Qed.
+
+Lemma base_ctx_step_val Ki e σ1 κ e2 σ2 ef :
+  base_step (fill_item Ki e) σ1 κ e2 σ2 ef → is_Some (to_val e).
+Proof.
+  destruct Ki; inversion_clear 1; decompose_Forall_hyps;
+    simplify_option_eq; by eauto.
+Qed.
+
+Lemma list_expr_val_eq_inv vl1 vl2 e1 e2 el1 el2 :
+  to_val e1 = None → to_val e2 = None →
+  map of_val vl1 ++ e1 :: el1 = map of_val vl2 ++ e2 :: el2 →
+  vl1 = vl2 ∧ el1 = el2.
+Proof.
+  revert vl2; induction vl1 as [|? vl1 IHvl1];
+    intros vl2; destruct vl2 as [|? vl2]; intros H1 H2; inversion 1.
+  - done.
+  - subst. by rewrite to_of_val in H1.
+  - subst. by rewrite to_of_val in H2.
+  - destruct (IHvl1 vl2); auto. split; f_equal; auto. by apply (inj of_val).
+Qed.
+
+Lemma fill_item_no_val_inj Ki1 Ki2 e1 e2 :
+  to_val e1 = None → to_val e2 = None →
+  fill_item Ki1 e1 = fill_item Ki2 e2 → Ki1 = Ki2.
+Proof.
+  destruct Ki1 as [| | |v1 vl1 el1| | | | | | | | | |],
+           Ki2 as [| | |v2 vl2 el2| | | | | | | | | |];
+  intros He1 He2 EQ; try discriminate; simplify_eq/=;
+    repeat match goal with
+    | H : to_val (of_val _) = None |- _ => by rewrite to_of_val in H
+    end; auto.
+  destruct (list_expr_val_eq_inv vl1 vl2 e1 e2 el1 el2); auto. congruence.
+Qed.
+
+Lemma shift_loc_assoc l n n' : l +ₗ n +ₗ n' = l +ₗ (n + n').
+Proof. rewrite /shift_loc /=. f_equal. lia. Qed.
+Lemma shift_loc_0 l : l +ₗ 0 = l.
+Proof. destruct l as [b o]. rewrite /shift_loc /=. f_equal. lia. Qed.
+
+Lemma shift_loc_assoc_nat l (n n' : nat) : l +ₗ n +ₗ n' = l +ₗ (n + n')%nat.
+Proof. rewrite /shift_loc /=. f_equal. lia. Qed.
+Lemma shift_loc_0_nat l : l +ₗ 0%nat = l.
+Proof. destruct l as [b o]. rewrite /shift_loc /=. f_equal. lia. Qed.
+
+Global Instance shift_loc_inj l : Inj (=) (=) (shift_loc l).
+Proof. destruct l as [b o]; intros n n' [= ?]; lia. Qed.
+
+Lemma shift_loc_block l n : (l +ₗ n).1 = l.1.
+Proof. done. Qed.
+
+Lemma lookup_init_mem σ (l l' : loc) (n : nat) :
+  l.1 = l'.1 → l.2 ≤ l'.2 < l.2 + n →
+  init_mem l n σ !! l' = Some (RSt 0, LitV LitPoison).
+Proof.
+  intros ?. destruct l' as [? l']; simplify_eq/=.
+  revert l. induction n as [|n IH]=> /= l Hl; [lia|].
+  assert (l' = l.2 ∨ l.2 + 1 ≤ l') as [->|?] by lia.
+  { by rewrite -surjective_pairing lookup_insert. }
+  rewrite lookup_insert_ne; last by destruct l; intros ?; simplify_eq/=; lia.
+  rewrite -(shift_loc_block l 1) IH /=; last lia. done.
+Qed.
+
+Lemma lookup_init_mem_ne σ (l l' : loc) (n : nat) :
+  l.1 ≠ l'.1 ∨ l'.2 < l.2 ∨ l.2 + n ≤ l'.2 →
+  init_mem l n σ !! l' = σ !! l'.
+Proof.
+  revert l. induction n as [|n IH]=> /= l Hl; auto.
+  rewrite -(IH (l +ₗ 1)); last (simpl; intuition lia).
+  apply lookup_insert_ne. intros ->; intuition lia.
+Qed.
+
+Definition fresh_block (σ : state) : block :=
+  let loclst : list loc := elements (dom σ : gset loc) in
+  let blockset : gset block := foldr (λ l, ({[l.1]} ∪.)) ∅ loclst in
+  fresh blockset.
+
+Lemma is_fresh_block σ i : σ !! (fresh_block σ,i) = None.
+Proof.
+  assert (∀ (l : loc) ls (X : gset block),
+    l ∈ ls → l.1 ∈ foldr (λ l, ({[l.1]} ∪.)) X ls) as help.
+  { induction 1; set_solver. }
+  rewrite /fresh_block /shift_loc /= -(not_elem_of_dom (D := gset loc)) -elem_of_elements.
+  move=> /(help _ _ ∅) /=. apply is_fresh.
+Qed.
+
+Lemma alloc_fresh n σ :
+  let l := (fresh_block σ, 0) in
+  let init := repeat (LitV $ LitInt 0) (Z.to_nat n) in
+  0 < n →
+  base_step (Alloc $ Lit $ LitInt n) σ [] (Lit $ LitLoc l) (init_mem l (Z.to_nat n) σ) [].
+Proof.
+  intros l init Hn. apply AllocS; first done.
+  - intros i. apply (is_fresh_block _ i).
+Qed.
+
+Lemma lookup_free_mem_ne σ l l' n : l.1 ≠ l'.1 → free_mem l n σ !! l' = σ !! l'.
+Proof.
+  revert l. induction n as [|n IH]=> l ? //=.
+  rewrite lookup_delete_ne; last congruence.
+  apply IH. by rewrite shift_loc_block.
+Qed.
+
+Lemma delete_free_mem σ l l' n :
+  delete l (free_mem l' n σ) = free_mem l' n (delete l σ).
+Proof.
+  revert l'. induction n as [|n IH]=> l' //=. by rewrite delete_commute IH.
+Qed.
+
+(** Closed expressions *)
+Lemma is_closed_weaken X Y e : is_closed X e → X ⊆ Y → is_closed Y e.
+Proof.
+  revert e X Y. fix FIX 1; intros e; destruct e=>X Y/=; try naive_solver.
+  - naive_solver set_solver.
+  - rewrite !andb_True. intros [He Hel] HXY. split; first by eauto.
+    rename select (list expr) into el.
+    induction el=>/=; naive_solver.
+  - rewrite !andb_True. intros [He Hel] HXY. split; first by eauto.
+    rename select (list expr) into el.
+    induction el=>/=; naive_solver.
+Qed.
+
+Lemma is_closed_weaken_nil X e : is_closed [] e → is_closed X e.
+Proof. intros. by apply is_closed_weaken with [], list_subseteq_nil. Qed.
+
+Lemma is_closed_subst X e x es : is_closed X e → x ∉ X → subst x es e = e.
+Proof.
+  revert e X. fix FIX 1; intros e; destruct e=> X /=; rewrite ?bool_decide_spec ?andb_True=> He ?;
+    repeat case_bool_decide; simplify_eq/=; f_equal;
+    try by intuition eauto with set_solver.
+  - case He=> _. clear He.
+    rename select (list expr) into el.
+    induction el=>//=. rewrite andb_True=>?.
+    f_equal; intuition eauto with set_solver.
+  - case He=> _. clear He.
+    rename select (list expr) into el.
+    induction el=>//=. rewrite andb_True=>?.
+    f_equal; intuition eauto with set_solver.
+Qed.
+
+Lemma is_closed_nil_subst e x es : is_closed [] e → subst x es e = e.
+Proof. intros. apply is_closed_subst with []; set_solver. Qed.
+
+Lemma is_closed_of_val X v : is_closed X (of_val v).
+Proof. apply is_closed_weaken_nil. induction v; simpl; auto. Qed.
+
+Lemma is_closed_to_val X e v : to_val e = Some v → is_closed X e.
+Proof. intros <-%of_to_val. apply is_closed_of_val. Qed.
+
+Lemma subst_is_closed X x es e :
+  is_closed X es → is_closed (x::X) e → is_closed X (subst x es e).
+Proof.
+  revert e X. fix FIX 1; intros e; destruct e=>X //=; repeat (case_bool_decide=>//=);
+    try naive_solver; rewrite ?andb_True; intros.
+  - set_solver.
+  - eauto using is_closed_weaken with set_solver.
+  - eapply is_closed_weaken; first done.
+    rename select binder into f.
+    rename select (list binder) into xl.
+    destruct (decide (BNamed x = f)), (decide (BNamed x ∈ xl)); set_solver.
+  - split; first naive_solver.
+    rename select (list expr) into el. induction el; naive_solver.
+  - split; first naive_solver.
+    rename select (list expr) into el. induction el; naive_solver.
+Qed.
+
+Lemma subst'_is_closed X b es e :
+  is_closed X es → is_closed (b:b:X) e → is_closed X (subst' b es e).
+Proof. destruct b; first done. apply subst_is_closed. Qed.
+
+(* Operations on literals *)
+Lemma lit_eq_state σ1 σ2 l1 l2 :
+  (∀ l, σ1 !! l = None ↔ σ2 !! l = None) →
+  lit_eq σ1 l1 l2 → lit_eq σ2 l1 l2.
+Proof. intros Heq. inversion 1; econstructor; eauto; eapply Heq; done. Qed.
+
+Lemma bin_op_eval_state σ1 σ2 op l1 l2 l' :
+  (∀ l, σ1 !! l = None ↔ σ2 !! l = None) →
+  bin_op_eval σ1 op l1 l2 l' → bin_op_eval σ2 op l1 l2 l'.
+Proof.
+  intros Heq. inversion 1; econstructor; eauto using lit_eq_state.
+Qed.
+
+(* Misc *)
+Lemma stuck_not_base_step σ e' κ σ' ef :
+  ¬base_step stuck_term σ e' κ σ' ef.
+Proof. inversion 1. Qed.
+
+(** Equality and other typeclass stuff *)
+Global Instance base_lit_dec_eq : EqDecision base_lit.
+Proof. solve_decision. Defined.
+Global Instance bin_op_dec_eq : EqDecision bin_op.
+Proof. solve_decision. Defined.
+Global Instance un_op_dec_eq : EqDecision order.
+Proof. solve_decision. Defined.
+
+Fixpoint expr_beq (e : expr) (e' : expr) : bool :=
+  let fix expr_list_beq el el' :=
+    match el, el' with
+    | [], [] => true
+    | eh::eq, eh'::eq' => expr_beq eh eh' && expr_list_beq eq eq'
+    | _, _ => false
+    end
+  in
+  match e, e' with
+  | Var x, Var x' => bool_decide (x = x')
+  | Lit l, Lit l' => bool_decide (l = l')
+  | Rec f xl e, Rec f' xl' e' =>
+    bool_decide (f = f') && bool_decide (xl = xl') && expr_beq e e'
+  | BinOp op e1 e2, BinOp op' e1' e2' =>
+    bool_decide (op = op') && expr_beq e1 e1' && expr_beq e2 e2'
+  | App e el, App e' el' | Case e el, Case e' el' =>
+    expr_beq e e' && expr_list_beq el el'
+  | Read o e, Read o' e' => bool_decide (o = o') && expr_beq e e'
+  | Write o e1 e2, Write o' e1' e2' =>
+    bool_decide (o = o') && expr_beq e1 e1' && expr_beq e2 e2'
+  | CAS e0 e1 e2, CAS e0' e1' e2' =>
+    expr_beq e0 e0' && expr_beq e1 e1' && expr_beq e2 e2'
+  | Alloc e, Alloc e' | Fork e, Fork e' => expr_beq e e'
+  | Free e1 e2, Free e1' e2' => expr_beq e1 e1' && expr_beq e2 e2'
+  | Ndnat, Ndnat => true
+  | _, _ => false
+  end.
+Lemma expr_beq_correct (e1 e2 : expr) : expr_beq e1 e2 ↔ e1 = e2.
+Proof.
+  revert e1 e2; fix FIX 1. intros e1 e2.
+    destruct e1 as [| | | |? el1| | | | | |? el1| |],
+             e2 as [| | | |? el2| | | | | |? el2| |]; simpl; try done;
+  rewrite ?andb_True ?bool_decide_spec ?FIX;
+  try (split; intro; [destruct_and?|split_and?]; congruence).
+  - match goal with |- context [?F el1 el2] => assert (F el1 el2 ↔ el1 = el2) end.
+    { revert el2. induction el1 as [|el1h el1q]; intros el2; destruct el2; try done.
+      specialize (FIX el1h). naive_solver. }
+    clear FIX. naive_solver.
+  - match goal with |- context [?F el1 el2] => assert (F el1 el2 ↔ el1 = el2) end.
+    { revert el2. induction el1 as [|el1h el1q]; intros el2; destruct el2; try done.
+      specialize (FIX el1h). naive_solver. }
+    clear FIX. naive_solver.
+Qed.
+Global Instance expr_dec_eq : EqDecision expr.
+Proof.
+ refine (λ e1 e2, cast_if (decide (expr_beq e1 e2))); by rewrite -expr_beq_correct.
+Defined.
+Global Instance val_dec_eq : EqDecision val.
+Proof.
+ refine (λ v1 v2, cast_if (decide (of_val v1 = of_val v2))); abstract naive_solver.
+Defined.
+
+Global Instance expr_inhabited : Inhabited expr := populate (Lit LitPoison).
+Global Instance val_inhabited : Inhabited val := populate (LitV LitPoison).
+
+#[warning="-redundant-canonical-projection"]
+Canonical Structure stateO := leibnizO state.
+#[warning="-redundant-canonical-projection"]
+Canonical Structure valO := leibnizO val.
+#[warning="-redundant-canonical-projection"]
+Canonical Structure exprO := leibnizO expr.
+
+(** Language *)
+Lemma lrust_lang_mixin : EctxiLanguageMixin of_val to_val fill_item base_step.
+Proof.
+  split; apply _ || eauto using to_of_val, of_to_val,
+    val_stuck, fill_item_val, fill_item_no_val_inj, base_ctx_step_val.
+Qed.
+Canonical Structure lrust_ectxi_lang := EctxiLanguage lrust_lang_mixin.
+#[warning="-redundant-canonical-projection"]
+Canonical Structure lrust_ectx_lang := EctxLanguageOfEctxi lrust_ectxi_lang.
+#[warning="-redundant-canonical-projection"]
+Canonical Structure lrust_lang := LanguageOfEctx lrust_ectx_lang.
+
+(* Lemmas about the language. *)
+Lemma stuck_irreducible K σ : irreducible (fill K stuck_term) σ.
+Proof.
+  apply: (irreducible_fill (K:=ectx_language.fill K)); first done.
+  apply prim_base_irreducible; unfold stuck_term.
+  - inversion 1.
+  - apply ectxi_language_sub_redexes_are_values.
+    intros [] ??; simplify_eq/=; eauto; discriminate_list.
+Qed.
+
+(* Define some derived forms *)
+Notation Lam xl e := (Rec BAnon xl e) (only parsing).
+Notation Let x e1 e2 := (App (Lam [x] e2) [e1]) (only parsing).
+Notation Seq e1 e2 := (Let BAnon e1 e2) (only parsing).
+Notation LamV xl e := (RecV BAnon xl e) (only parsing).
+Notation LetCtx x e2 := (AppRCtx (LamV [x] e2) [] []).
+Notation SeqCtx e2 := (LetCtx BAnon e2).
+Notation Skip := (Seq (Lit LitPoison) (Lit LitPoison)).
+Coercion lit_of_bool : bool >-> base_lit.
+Notation If e0 e1 e2 := (Case e0 (@cons expr e2 (@cons expr e1 (@nil expr)))) (only parsing).
