nola/rust_lang/notation.v
@@ -1,0 +1,105 @@
+From nola.rust_lang Require Export lang.
+From iris.prelude Require Import options.
+
+Coercion LitInt : Z >-> base_lit.
+Coercion LitLoc : loc >-> base_lit.
+
+Coercion App : expr >-> Funclass.
+Coercion of_val : val >-> expr.
+
+Coercion Var : string >-> expr.
+
+Notation "[ ]" := (@nil expr) : expr_scope.
+Notation "[ x ]" := (@cons expr x%E (@nil expr)) : expr_scope.
+Notation "[ x1 ; x2 ; .. ; xn ]" :=
+  (@cons expr x1%E (@cons expr x2%E
+        (..(@cons expr xn%E (@nil expr))..))) : expr_scope.
+
+(* No scope for the values, does not conflict and scope is often not inferred
+properly. *)
+Notation "# l" := (LitV l%Z%V%L) (at level 8, format "# l").
+Notation "# l" := (Lit l%Z%V%L) (at level 8, format "# l") : expr_scope.
+
+(** Syntax inspired by Coq/Ocaml. Constructions with higher precedence come
+    first. *)
+Notation "'case:' e0 'of' el" := (Case e0%E el%E)
+  (at level 102, e0, el at level 150) : expr_scope.
+Notation "'if:' e1 'then' e2 'else' e3" := (If e1%E e2%E e3%E)
+  (only parsing, at level 102, e1, e2, e3 at level 150) : expr_scope.
+Notation "☠" := LitPoison : val_scope.
+Notation "! e" := (Read Na1Ord e%E) (at level 9, format "! e") : expr_scope.
+Notation "!ˢᶜ e" := (Read ScOrd e%E) (at level 9, format "!ˢᶜ e") : expr_scope.
+Notation "e1 + e2" := (BinOp PlusOp e1%E e2%E)
+  (at level 50, left associativity) : expr_scope.
+Notation "e1 - e2" := (BinOp MinusOp e1%E e2%E)
+  (at level 50, left associativity) : expr_scope.
+Notation "e1 ≤ e2" := (BinOp LeOp e1%E e2%E)
+  (at level 70) : expr_scope.
+Notation "e1 < e2" := (e1+#1 ≤ e2)%E
+  (at level 70) : expr_scope.
+Notation "e1 = e2" := (BinOp EqOp e1%E e2%E)
+  (at level 70) : expr_scope.
+(* The unicode ← is already part of the notation "_ ← _; _" for bind. *)
+Notation "e1 <-ˢᶜ e2" := (Write ScOrd e1%E e2%E)
+  (at level 80) : expr_scope.
+Notation "e1 <- e2" := (Write Na1Ord e1%E e2%E)
+  (at level 80) : expr_scope.
+Notation "'rec:' f xl := e" := (Rec f%binder xl%binder e%E)
+  (at level 102, f, xl at level 1, e at level 200) : expr_scope.
+Notation "'rec:' f xl := e" := (locked (RecV f%binder xl%binder e%E))
+  (at level 102, f, xl at level 1, e at level 200) : val_scope.
+Notation "e1 +ₗ e2" := (BinOp OffsetOp e1%E e2%E)
+  (at level 50, left associativity) : expr_scope.
+
+(** Derived notions. The notations for let and seq are stated
+explicitly instead of relying on the Notations Let and Seq as defined
+above. This is needed because App is now a coercion, and these
+notations are otherwise not pretty printed back accordingly. *)
+
+Notation "λ: xl , e" := (Lam xl%binder e%E)
+  (at level 102, xl at level 1, e at level 200) : expr_scope.
+Notation "λ: xl , e" := (locked (LamV xl%binder e%E))
+  (at level 102, xl at level 1, e at level 200) : val_scope.
+
+Notation "'fnrec:' f xl := e" := (rec: f (BNamed "return"::xl) := e)%E
+  (at level 102, f, xl at level 1, e at level 200) : expr_scope.
+Notation "'fnrec:' f xl := e" := (rec: f (BNamed "return"::xl) := e)%V
+  (at level 102, f, xl at level 1, e at level 200) : val_scope.
+Notation "'fn:' xl := e" := (fnrec: <> xl := e)%E
+  (at level 102, xl at level 1, e at level 200) : expr_scope.
+Notation "'fn:' xl := e" := (fnrec: <> xl := e)%V
+  (at level 102, xl at level 1, e at level 200) : val_scope.
+Notation "'return:'" := "return" : expr_scope.
+
+Notation "'let:' x := e1 'in' e2" :=
+  ((Lam (@cons binder x%binder nil) e2%E) (@cons expr e1%E nil))
+  (at level 102, x at level 1, e1, e2 at level 150) : expr_scope.
+Notation "e1 ;; e2" := (let: <> := e1 in e2)%E
+  (at level 100, e2 at level 200, format "e1  ;;  e2") : expr_scope.
+(* These are not actually values, but we want them to be pretty-printed. *)
+Notation "'let:' x := e1 'in' e2" :=
+  (LamV (@cons binder x%binder nil) e2%E (@cons expr e1%E nil))
+  (at level 102, x at level 1, e1, e2 at level 150) : val_scope.
+Notation "e1 ;; e2" := (let: <> := e1 in e2)%V
+  (at level 100, e2 at level 200, format "e1  ;;  e2") : val_scope.
+
+Notation "'letcont:' k xl := e1 'in' e2" :=
+  ((Lam (@cons binder k%binder nil) e2%E) [Rec k%binder xl%binder e1%E])
+  (at level 102, k, xl at level 1, e1, e2 at level 150) : expr_scope.
+Notation "'withcont:' k1 ':' e1 'cont:' k2 xl := e2" :=
+  ((Lam (@cons binder k1%binder nil) e1%E) [Rec k2%binder ((fun _ : eq k1%binder k2%binder => xl%binder) eq_refl) e2%E])
+  (only parsing, at level 151, k1, k2, xl at level 1, e2 at level 150) : expr_scope.
+
+Notation "'call:' f args → k" := (f (@cons expr (λ: ["_r"], k ["_r"]) args))%E
+  (only parsing, at level 102, f, args, k at level 1) : expr_scope.
+Notation "'letcall:' x := f args 'in' e" :=
+  (letcont: "_k" [ x ] := e in call: f args → "_k")%E
+  (at level 102, x, f, args at level 1, e at level 150) : expr_scope.
+
+(* These notations unfortunately do not print.  Also, I don't think
+   we would even want them to print in general.
+   TODO: Introduce a Definition. *)
+Notation "e1 '<-{Σ' i } '()'" := (e1 <- #i)%E
+  (only parsing, at level 80) : expr_scope.
+Notation "e1 '<-{Σ' i } e2" := (e1 <-{Σ i} () ;; e1+ₗ#1 <- e2)%E
+  (at level 80, format "e1 <-{Σ  i }  e2") : expr_scope.
